Added TaggedGLS and skeleton for performance guarantee

ironfleet/src/Dafny/Distributed/Protocol/Lock/PerformanceProof/PerformanceProof.i.dfy
@@ -1,11 +1,37 @@
 include "../../../Services/Lock/LockTaggedDistributedSystem.i.dfy"
+  include "TaggedGLS.i.dfy"
 
 module PerformanceProof_i {
 import opened LockTaggedDistributedSystem_i
+  import opened TaggedGLS_i
 
-predicate dummy(config:ConcreteConfiguration, tdb:seq<TaggedDS_State>)
+predicate SingleGLSPerformanceAssumption(tgls:TaggedGLS_State)
 {
-  false
+  tgls.tls.t_environment.nextStep.LEnvStepHostIos? ==> tgls.tls.t_environment.nextStep.actor in tgls.tls.t_servers
 }
+
+predicate GLSPerformanceAssumption(tglb:seq<TaggedGLS_State>)
+{
+  forall tgls :: tgls in tglb ==> SingleGLSPerformanceAssumption(tgls)
+}
+
+predicate SingleGLSPerformanceGuarantee(gls:TaggedGLS_State)
+{
+  forall pkt :: pkt in gls.tls.t_environment.sentPackets &&
+    pkt.msg.v == Locked(|gls.tls.config|) ==> pkt.msg.pr == PerformanceReport(0, 0)
+}
+
+predicate GLSPerformanceGuarantee(tglb:seq<TaggedGLS_State>)
+{
+  forall tgls :: tgls in tglb ==> SingleGLSPerformanceGuarantee(tgls)
+}
+
+lemma PerformanceGuaranteeHolds(config:Config, tglb:seq<TaggedGLS_State>)
+  requires ValidTaggedGLSBehavior(tglb, config)
+  requires GLSPerformanceAssumption(tglb)
+  ensures GLSPerformanceGuarantee(tglb)
+{
   
+}
+
 }
