ironfleet/src/Dafny/Distributed/Protocol/Lock/PerformanceProof/TaggedGLS.i.dfy
@@ -1,0 +1,99 @@
+include "../Node.i.dfy"
+  include "../RefinementProof/DistributedSystem.i.dfy"
+include "../../../Services/Lock/LockTaggedDistributedSystem.i.dfy"
+
+module TaggedGLS_i {
+import opened Protocol_Node_i
+import opened DistributedSystem_i
+import opened LockTaggedDistributedSystem_i
+
+type TaggedNode = TaggedType<Node>
+  
+datatype TaggedLS_State = TaggedLS_State(
+  config:ConcreteConfiguration,
+  t_environment:TaggedLEnvironment<EndPoint, LockMessage, HostStep>,
+  t_servers:map<EndPoint,TaggedNode>
+  )
+
+datatype TaggedGLS_State = TaggedGLS_State(
+  tls:TaggedLS_State,
+  history:seq<EndPoint>
+  )
+
+  function UntagLSServers(t_servers: map<EndPoint, TaggedNode>) : map<EndPoint, Node>
+  {
+    map id | id in t_servers :: t_servers[id].v
+  }
+  
+
+  function UntagLS_State(tds:TaggedLS_State) : LS_State
+  {
+    LS_State(
+      UntagLEnvironment(tds.t_environment),
+      UntagLSServers(tds.t_servers))
+  }
+
+  predicate TLS_Init(tls: TaggedLS_State, config:Config)
+    reads *
+  {
+    LS_Init(UntagLS_State(tls), config)
+      && LEnvironment_Init(tls.t_environment)
+      && forall id :: id in tls.t_servers ==> tls.t_servers[id].pr == PerformanceReport(0, 0)
+  }
+
+  predicate TLS_NextOneServer(tls: TaggedLS_State, tls': TaggedLS_State, id:EndPoint, ios:seq<TaggedLIoOp<EndPoint, LockMessage>>)
+    requires id in tls.t_servers;
+    reads *
+  {
+    LS_NextOneServer(UntagLS_State(tls), UntagLS_State(tls'), id, UntagLIoOpSeq(ios))
+      && tls'.t_servers[id].pr == PerfMax(GetReceivePRs(ios) + [tls.t_servers[id].pr])
+      && (forall t_io :: t_io in ios && t_io.LIoOpSend? ==> t_io.s.msg.pr == tls'.t_servers[id].pr)
+      && tls'.t_servers == tls.t_servers[id := tls'.t_servers[id]]
+  }
+
+  predicate TLS_Next(tls:TaggedLS_State, tls': TaggedLS_State)
+    reads *
+  {
+    tls.config == tls'.config
+    && LS_Next(UntagLS_State(tls), UntagLS_State(tls'))
+    && LEnvironment_Next(tls.t_environment, tls'.t_environment)
+    && if tls.t_environment.nextStep.LEnvStepHostIos? && tls.t_environment.nextStep.actor in tls.t_servers then
+           TLS_NextOneServer(tls, tls', tls.t_environment.nextStep.actor, tls.t_environment.nextStep.ios)
+       else
+        tls'.t_servers == tls.t_servers
+
+        && (if tls.t_environment.nextStep.LEnvStepHostIos? then
+            && (forall t_io :: t_io in tls.t_environment.nextStep.ios && t_io.LIoOpSend? ==> t_io.s.msg.pr == PerformanceReport(0, 0))
+            else
+            true)
+  }
+
+  predicate TGLS_Init(tgls:TaggedGLS_State, config:Config)
+    reads *
+  {
+    TLS_Init(tgls.tls, config)
+      && tgls.history == [config[0]]
+  }
+
+  predicate TGLS_Next(tgls:TaggedGLS_State, tgls':TaggedGLS_State)
+    reads *
+  {
+    TLS_Next(tgls.tls, tgls'.tls)
+      && (if tgls.tls.t_environment.nextStep.LEnvStepHostIos? && tgls.tls.t_environment.nextStep.actor in tgls.tls.t_servers
+      && NodeGrant(tgls.tls.t_servers[tgls.tls.t_environment.nextStep.actor].v, tgls'.tls.t_servers[tgls.tls.t_environment.nextStep.actor].v, UntagLIoOpSeq(tgls.tls.t_environment.nextStep.ios))
+      && tgls.tls.t_servers[tgls.tls.t_environment.nextStep.actor].v.held && tgls.tls.t_servers[tgls.tls.t_environment.nextStep.actor].v.epoch < 0xFFFF_FFFF_FFFF_FFFF then
+      tgls'.history == tgls.history + [tgls.tls.t_servers[tgls.tls.t_environment.nextStep.actor].v.config[(tgls.tls.t_servers[tgls.tls.t_environment.nextStep.actor].v.my_index + 1) % |tgls.tls.t_servers[tgls.tls.t_environment.nextStep.actor].v.config|]]
+      else
+        tgls'.history == tgls.history
+        )
+  }
+
+  predicate ValidTaggedGLSBehavior(tglb:seq<TaggedGLS_State>, config:Config)
+    reads *
+  {
+      && TGLS_Init(tglb[0], config)
+      && (forall i :: i >= 0 ==> TGLS_Next(tglb[i], tglb[i+1]))
+  }
+
+
+}
